Redefine traces and reachability

Trace.lean
@@ -3,16 +3,34 @@ import «State»
 import «Tokens»
 import «Swap»
 
-inductive Trace (c: Config): State → Type where
-  | empty (accs: AccountSet) 
-    (h: ∀(a: Account) (m: MintedTok), accs a m = 0): 
-      Trace c ⟨accs, AMMSet.empty⟩
+/- Tx c init s is the type of all possible sequences of transactions
+  that would result in s, starting from state init and using configuration c -/
+inductive Tx (c: Config) (init: State): State → Type where
+  | empty: Tx c init init
 
-  | dep0 (s: State) (rs: Trace c s) (d: Deposit0.Valid s): 
-      Trace c (Deposit0.apply d)
+  | dep0 (s': State) (rs: Tx c init s') (d: Deposit0.Valid s'): 
+      Tx c init (Deposit0.apply d)
 
-  | swap (s: State) (rs: Trace c s) (sw: Swap.Valid c s):
-      Trace c (Swap.apply sw)
+  | swap (s': State) (rs: Tx c init s') (sw: Swap.Valid c s'):
+      Tx c init (Swap.apply sw)
+
+def reachableInit (s: State): Prop :=
+  (s.amms = AMMSet.empty ∧ ∀ (a: Account) (m: MintedTok), s.accs a m = 0)
+
+def reachable (c: Config) (s: State): Prop :=
+  ∃ (init: State) (tx: Tx c init s), reachableInit init
+
+structure Reachable (c: Config) (s: State) where
+  init: State
+  tx: Tx c init s
+  init_amms: init.amms = AMMSet.empty
+  init_accs: ∀ (a: Account) (m: MintedTok), init.accs a m = 0
+
+def concat {c: Config} {init s' s'': State} 
+(t1: Tx c init s') (t2: Tx c s' s''): Tx c init s'' := match t2 with
+  | Tx.empty => t1
+  | Tx.dep0 ds rs d => Tx.dep0 ds (concat t1 rs) d
+  | Tx.swap ds rs sw => Tx.swap ds (concat t1 rs) sw
 
 /-
 Proof that 
@@ -20,32 +38,42 @@ m ∈ (Trace c s).state.amms.map.supp → supply m > 0
 
 by induction
 empty (base case): hypothesis is a contradiction
-dep0: trivial
+dep0: trivial by cases on the deposited tokens:
+      if the pair is the same, then the supply is positive.
+      if the pair isn't the same, the supply is the same as
+      before and we can use IH.
 swap: use IH. 
       swaps don't change minted token supplies
 -/
-theorem AMMimpSupply 
-(t: Trace c s) (t0 t1: AtomicTok) (h: s.amms.f t0 t1 ≠ 0)
-: 0 < s.supply (AtomicTok.toMint (AMMSet.exists_imp_dif h)) := by
-  induction t with
-  | empty accs _ => 
-    exfalso
-    simp [AMMSet.empty] at h
 
-  | dep0 s' _ d ih =>
+theorem AMMimpSupplyProp
+{c: Config} {s: State} (r: reachable c s) {t0 t1: AtomicTok}
+(h: s.amms.f t0 t1 ≠ 0)
+: 0 < s.supply (AtomicTok.toMint (AMMSet.exists_imp_dif h)) := by
+  have ⟨init, tx, ⟨init_amms, init_accs⟩⟩ := r
+  induction tx with
+  | empty => 
+      exfalso
+      simp [init_amms, AMMSet.empty] at h
+
+  | dep0 sprev tail d ih =>
     apply @Decidable.byCases ((AtomicTok.toMint (AMMSet.exists_imp_dif h))=(AtomicTok.toMint d.hdif))
     . intro eq; rw [eq]
       simp [Deposit0.apply, State.supply]
-      rw [AccountSet.supply_addb_same (((s'.accs.subb d.a d.t0 d.r0).subb d.a d.t1 d.r1)) (AtomicTok.toMint d.hdif) d.a d.r0]
+      rw [AccountSet.supply_addb_same (((sprev.accs.subb d.a d.t0 d.r0).subb d.a d.t1 d.r1)) (AtomicTok.toMint d.hdif) d.a d.r0]
       apply NNReal.neq_zero_imp_gt
       exact NNReal.pos_imp_add_pos d.r0 _ (d.r0.coe_nnreal_pos)
-
+    
     . intro neq
       simp [neq]
       simp [AtomicTok.toMint_diff neq] at h
-      exact ih h
+      have re: reachable c sprev := by
+        exists init; exists tail
+      exact ih re h
   
-  | swap s' _ sw ih =>
-    rw [Swap.mintedSupply]
-    have h' := Swap.amm_in_apply h
-    exact ih h'
+  | swap sprev tail sw ih =>
+      rw [Swap.mintedSupply]
+      have h' := Swap.amm_in_apply h
+      have re: reachable c sprev := by
+        exists init; exists tail
+      exact ih re h'
